tests/avgvelocity.cdf
@@ -8,6 +8,6 @@ node avgvelocity (delta:int, sec:bool) returns (v:int);
 let
   h :: base = 0 fby (v:int);
   v :: base = merge (sec:bool) ((((r:int) when sec) / (t:int) : int)) ((h:int) whennot sec);
-  t :: base on sec = counter ((0:int) when sec, (1:int) when sec, (false:bool) when sec);
-  r :: base = counter ((0:int), (delta:int), (false:bool));
+  t :: base on sec = counter ((0:int) when sec, (1:int) when sec, (false:bool) when sec) : int;
+  r :: base = counter ((0:int), (delta:int), (false:bool)) : int;
 tel;
